trying new definition of indistinguishability

coq/full/Indistinguishability.v
@@ -1,3 +1,4 @@
+Require Import Classical.
 Require Import Program.Tactics.
 Require Import MyTactics.
 Require Import LabelAlgebra.
@@ -14,13 +15,15 @@ Context (L : Type)
 Fixpoint atom_LPequiv a1 a2 : Prop :=
   match a1, a2 with
     | Atom v1 l1, Atom v2 l2 =>
-      ((l1 ⊑ l \/ l2 ⊑ l) -> (value_LPequiv v1 v2 /\ l1 =L l2)) /\
-      ((l ⊑ l1 /\ l ⊑ l2) ->
+      ((l1 ⊑ l \/ l2 ⊑ l) /\
+       value_LPequiv v1 v2 /\ l1 =L l2) \/
+      (l ⊑ l1 /\ l ⊑ l2 /\ ~ l =L l1 /\ ~ l =L l2 /\
        match v1, v2 with
          | VNat n1, VNat n2 => P v1 v2
          | VClos e1 t1, VClos e2 t2 => value_LPequiv v1 v2
          | _, _ => True
-       end)
+       end) \/
+      (~ l ⊑ l1 /\ ~ l1 ⊑ l /\ ~ l ⊑ l2 /\ ~ l2 ⊑ l)
   end
 with value_LPequiv v1 v2 : Prop :=
        match v1, v2 with
@@ -33,5 +36,48 @@ with value_LPequiv v1 v2 : Prop :=
 
 Definition env_LPequiv : env L -> env L -> Prop :=
   list_forall2 atom_LPequiv.
+
+Lemma atom_value_env_LPequiv_refl :
+  (forall a, atom_LPequiv a a) /\
+  (forall v, value_LPequiv v v) /\
+  (forall e, env_LPequiv e e).
+Proof.
+  apply atom_value_env_mutind.
+  - intros v Hv l1.
+    assert (H1: l1 ⊑ l \/ ~ l1 ⊑ l) by apply classic.
+    assert (H2: l ⊑ l1 \/ ~ l ⊑ l1) by apply classic.
+    destruct v as [b | n | e t];
+      (destruct H1 as [H1 | H1]; destruct H2 as [H2 | H2]; [
+         left; auto |
+         left; auto |
+         right; left; splits; auto |
+         right; right; auto
+       ]).
+  - intros b.
+    unfold value_LPequiv. auto.
+  - intros n.
+    unfold value_LPequiv. auto.
+  - intros e He t.
+    unfold value_LPequiv. auto.
+  - intros e Ha.
+    unfold env_LPequiv.
+    induction e as [| a e'].
+    + reflexivity.
+    + split.
+      * apply (Ha 0). reflexivity.
+      * apply IHe'. intros. apply (Ha (S n)). auto.
+Qed.
+
+Lemma atom_LPequiv_refl :
+  forall a, atom_LPequiv a a.
+Proof. apply atom_value_env_LPequiv_refl. Qed.
+
+Lemma value_LPequiv_refl :
+  forall v, value_LPequiv v v.
+Proof. apply atom_value_env_LPequiv_refl. Qed.
+
+Lemma env_LPequiv_refl :
+  forall e, env_LPequiv e e.
+Proof. apply atom_value_env_LPequiv_refl. Qed.
 
 End Indistinguishability.
